ver3_less_complex/Lemmas.dfy
@@ -8,7 +8,7 @@ module M_Lemma {
     import opened M_System
 
     lemma{:axiom} Axiom_Byz_Constraints()
-    ensures |Adversary_Nodes| <= f(|Honest_Nodes| + |Adversary_Nodes|)
+    ensures |Adversary_Nodes| <= f(|All_Nodes|)
     ensures Adversary_Nodes * Honest_Nodes == {}
 
     lemma{:axiom} Axiom_Common_Constraints()
@@ -17,54 +17,93 @@ module M_Lemma {
     lemma{:axiom} NoOuterClient()
     ensures forall cert : Signature :: cert.signer in All_Nodes
 
+    lemma{:axiom} LemmaHonestNodeOnlyVotePrepareOnceInOneView(ss : SystemState)
+    ensures forall s1 : Signature, s2 : Signature | 
+                                                    && IsHonest(ss, s1.signer)
+                                                    && IsHonest(ss, s2.signer)
+                                                    && s1.signer == s2.signer
+                                                    && s1.block == s2.block
+                                                    && s1.mType == s2.mType
+                                                  ::
+                                                    s1.viewNum == s2.viewNum
+
     /**
      * Lemma: for 2 valid certificate, if they are not conflict, then their coressponding view number should be different
      */
-    lemma LemmaViewDiffOnConflictCertificate(cert1 : Cert, cert2 : Cert)
-    requires cert1.Cert? && cert2.Cert?
-    requires cert1.cType == cert2.cType
-    requires ValidQC(cert1) && ValidQC(cert2)
-    requires cert1.block.Block? && cert2.block.Block?
-    requires !NoConflict(cert1.block, cert2.block)
-    ensures cert1.viewNum != cert2.viewNum
-    {
-        // var votesInCert1 := getVotesInValidQC(cert1);
-        // var voterInCert1 := getMajoritySignerInValidQC(cert1);
-
-        // var votesInCert2 := getVotesInValidQC(cert2);
-        // var voterInCert2 := getMajoritySignerInValidQC(cert2);
-
-        // assert voterInCert1 <= All_Nodes && voterInCert2 <= All_Nodes;
-
-        // assert |Adversary_Nodes| <= f(|All_Nodes|);
-        assert |All_Nodes| > 0 by {
-            Axiom_Common_Constraints();
-        }
-
-        // assert voterInCert1 * voterInCert2 * Honest_Nodes != {} by {
-        //     LemmaTwoQuorumIntersection(
-        //         All_Nodes,
-        //         Adversary_Nodes,
-        //         voterInCert1,
-        //         voterInCert2
-        //     );
-        // }
-    }
-
-    lemma LemmaViewDiffOnConflictCertificate2(ss : SystemState)
+    lemma LemmaViewDiffOnConflictCertificatePrepare(ss : SystemState)
+    // requires All_Nodes != {}
     requires ValidSystemState(ss)
-    ensures forall r1, r2, cert1, cert2 | && r1 in ss.nodeStates.Keys
-                                          && r2 in ss.nodeStates.Keys
-                                          && IsHonest(ss, r1)
+    ensures forall r1, r2, cert1, cert2 | && IsHonest(ss, r1)
                                           && IsHonest(ss, r2)
                                           && cert1 == ss.nodeStates[r1].prepareQC && cert1.Cert? 
                                           && cert2 == ss.nodeStates[r2].prepareQC && cert2.Cert?
                                           && cert1.block.Block?
                                           && cert2.block.Block?
                                           && !NoConflict(cert1.block, cert2.block)
-                                        ::cert1.viewNum != cert2.viewNum
+                                        ::
+                                          cert1.viewNum != cert2.viewNum
+
     {
+        assert ss.nodeStates.Keys - ss.adversary.byz_nodes != {};
+        var r1 :| IsHonest(ss, r1);
+        var r2 :| IsHonest(ss, r2);
+        var cert1 :| && cert1 == ss.nodeStates[r1].prepareQC;
+        var cert2 :| && cert2 == ss.nodeStates[r2].prepareQC;
+
+        // var r1, r2, cert1, cert2 :| && IsHonest(ss, r1)
+        //                             && IsHonest(ss, r2)
+        //                             && cert1 == ss.nodeStates[r1].prepareQC
+        //                             && cert2 == ss.nodeStates[r2].prepareQC;
+                                    // && cert1 == ss.nodeStates[r1].prepareQC && cert1.Cert? 
+                                    // && cert2 == ss.nodeStates[r2].prepareQC && cert2.Cert?
+                                    // && cert1.block.Block?
+                                    // && cert2.block.Block?
+                                    // && !NoConflict(cert1.block, cert2.block);
+        assume cert1.Cert?;
+        assume cert2.Cert?;
+        assume cert1.block.Block?;
+        assume cert2.block.Block?;
+        assume !NoConflict(cert1.block, cert2.block);
+        calc {
+            !NoConflict(cert1.block, cert2.block);
+            ==>
+            cert1.block != cert2.block;
+        }
         
-    }
+        var signers1 := getMajoritySignerInValidQC(cert1);
+        var signers2 := getMajoritySignerInValidQC(cert2);
+        assert signers1 * signers2 * Honest_Nodes != {} by
+        {
+            Axiom_Byz_Constraints();
+            LemmaTwoQuorumIntersection(All_Nodes, Adversary_Nodes, signers1, signers2);
+        }
+        var replica :| replica in signers1 * signers2 * Honest_Nodes;
+        var sign1 :| && sign1 in cert1.signatures
+                     && sign1.signer == replica;
+        var sign2 :| && sign2 in cert2.signatures
+                     && sign2.signer == replica;
+        assert sign1 != sign2;
+        calc {
+            sign1 != sign2
+            ==>
+            cert1.viewNum != cert2.viewNum;
+        }
+    } 
+
+    /**
+     * Lemma: for 2 valid certificate, if they are not conflict, then their coressponding view number should be different
+     */
+    lemma LemmaViewDiffOnConflictCertificateCommit(ss : SystemState)
+    // requires All_Nodes != {}
+    requires ValidSystemState(ss)
+    ensures forall r1, r2, cert1, cert2 | && IsHonest(ss, r1)
+                                          && IsHonest(ss, r2)
+                                          && cert1 == ss.nodeStates[r1].commitQC && cert1.Cert? 
+                                          && cert2 == ss.nodeStates[r2].commitQC && cert2.Cert?
+                                          && cert1.block.Block?
+                                          && cert2.block.Block?
+                                          && !NoConflict(cert1.block, cert2.block)
+                                        ::
+                                          cert1.viewNum != cert2.viewNum
 
 }
